Tests.lean
@@ -3,4 +3,4 @@ import Tests.Validation
 import Tests.Operation
 import Tests.NormalForm
 import Tests.Execution
-import Tests.DataModel
+import Tests.Algorithms.ExecutionUngrouped
